theories/TRAKHTENBROT/fo_terms.v
@@ -25,6 +25,8 @@ Set Implicit Arguments.
 
 (** Then first order terms with signature *)
 
+Local Hint Resolve in_vec_list in_vec_pos.
+
 Section first_order_terms.
 
   Variable (var sym : Type)        (* a type of variables and symbols *)
@@ -87,7 +89,7 @@ Section first_order_terms.
         end Ht.
     Proof. destruct Ht; reflexivity. Qed.
 
-    Definition fo_term_rect t : P t.
+    Definition fo_term_rect' t : P t.
     Proof. apply Fix_IHP with (1 := Acc_sub_fo_term t). Defined.
 
     Hypothesis IHP_ext : forall s v f g, (forall y H, f y H = g y H) -> @IHP s v f = IHP v g.
@@ -98,10 +100,10 @@ Section first_order_terms.
       intros [] f g H; auto; apply IHP_ext; auto.
     Qed.
 
-    Theorem fo_term_rect_fix s v : 
-            fo_term_rect (@in_fot s v) = @IHP s v (fun t _ => fo_term_rect t).
+    Theorem fo_term_rect_fix' s v : 
+            fo_term_rect' (@in_fot s v) = @IHP s v (fun t _ => fo_term_rect' t).
     Proof.
-      unfold fo_term_rect at 1.
+      unfold fo_term_rect' at 1.
       rewrite Fix_IHP_fix.
       apply IHP_ext.
       intros; apply Fix_IHP_Acc_irr.
@@ -109,8 +111,8 @@ Section first_order_terms.
 
   End fo_term_rect.
 
-  Definition fo_term_rec (P : _ -> Set) := @fo_term_rect P.
-  Definition fo_term_ind (P : _ -> Prop) := @fo_term_rect P.
+  Definition fo_term_rec' (P : _ -> Set) := @fo_term_rect' P.
+  Definition fo_term_ind' (P : _ -> Prop) := @fo_term_rect' P.
 
   Section fo_term_pos_rect.
 
@@ -127,6 +129,10 @@ Section first_order_terms.
       end.
 
   End fo_term_pos_rect.
+
+  Definition fo_term_rect (P : _ -> Type) := @fo_term_pos_rect P.
+  Definition fo_term_rec (P : _ -> Set) := @fo_term_rect P.
+  Definition fo_term_ind (P : _ -> Prop) := @fo_term_rect P.
  
   Section fo_term_recursion.
 
@@ -139,7 +145,7 @@ Section first_order_terms.
 
     Definition fo_term_recursion : fo_term -> X.
     Proof.
-      induction 1 as [ x | s v IHv ] using fo_term_pos_rect.
+      induction 1 as [ x | s v IHv ].
       + exact (F0 x).
       + apply (@F s v), vec_set_pos, IHv.
     Defined.
@@ -160,31 +166,50 @@ Section first_order_terms.
   (** We can now define eg the size of terms easily with the
       corresponding fixpoint equation *)
 
-  Fixpoint fo_term_size' c t :=
+  Fixpoint fo_term_size c t :=
     match t with
       | in_var _    => 1
-      | @in_fot s v => c s + vec_sum (vec_map (fo_term_size' c) v)
+      | @in_fot s v => c s + vec_sum (vec_map (fo_term_size c) v)
     end.
 
-  Definition fo_term_size (c : sym -> nat) : fo_term -> nat.
+  Fact fo_term_size_fix_0 c x : fo_term_size c (in_var x) = 1.
+  Proof. trivial. Qed.
+  
+  Fact fo_term_size_fix_1 c s v :
+         fo_term_size c (@in_fot s v) = c s + vec_sum (vec_map (fo_term_size c) v).
+  Proof. trivial. Qed.
+
+  (*
+
+  Definition fo_term_size' (c : sym -> nat) : fo_term -> nat.
   Proof.
     induction 1 as [ _ | s _ w ] using fo_term_recursion.
     + exact 1.
     + exact (c s+vec_sum w).
   Defined.
 
-  Fact fo_term_size_fix_0 c x : fo_term_size c (in_var x) = 1.
+  Fact fo_term_size_fix_0' c x : fo_term_size' c (in_var x) = 1.
   Proof. apply fo_term_recursion_fix_0. Qed.
   
-  Fact fo_term_size_fix_1 c s v :
-         fo_term_size c (@in_fot s v) = c s + vec_sum (vec_map (fo_term_size c) v).
+  Fact fo_term_size_fix_1' c s v :
+         fo_term_size' c (@in_fot s v) = c s + vec_sum (vec_map (fo_term_size' c) v).
   Proof. apply fo_term_recursion_fix_1. Qed.
 
-  Fixpoint fo_term_vars' t : list var :=
+  *)
+
+  Fixpoint fo_term_vars t :=
     match t with 
       | in_var x    => x::nil
-      | @in_fot s v => concat (vec_list (vec_map fo_term_vars' v))
+      | @in_fot s v => concat (vec_list (vec_map fo_term_vars v))
     end.
+
+  Fact fo_term_vars_fix_0 x : fo_term_vars (in_var x) = x :: nil.
+  Proof. trivial. Qed.
+
+  Fact fo_term_vars_fix_1 s v : fo_term_vars (@in_fot s v) = flat_map fo_term_vars (vec_list v).
+  Proof. simpl; rewrite vec_list_vec_map, <- flat_map_concat_map; auto. Qed.
+
+  (*
 
   Definition fo_term_vars : fo_term -> list var.
   Proof.
@@ -202,6 +227,22 @@ Section first_order_terms.
   Fact fo_term_vars_fix_1 s v : fo_term_vars (@in_fot s v) = flat_map fo_term_vars (vec_list v).
   Proof. rewrite fo_term_vars_fix_2, vec_list_vec_map, <- flat_map_concat_map; auto. Qed.
 
+  *)
+
+  Fixpoint fo_term_syms t :=
+    match t with 
+      | in_var x    => nil
+      | @in_fot s v => s::concat (vec_list (vec_map fo_term_syms v))
+    end.
+
+  Fact fo_term_syms_fix_0 x : fo_term_syms (in_var x) = nil.
+  Proof. trivial. Qed.
+
+  Fact fo_term_syms_fix_1 s v : fo_term_syms (@in_fot s v) = s::flat_map fo_term_syms (vec_list v).
+  Proof. simpl; rewrite vec_list_vec_map, <- flat_map_concat_map; auto. Qed.
+
+   (*
+
   Definition fo_term_syms : fo_term -> list sym.
   Proof.
     induction 1 as [ x | s _ w ] using fo_term_recursion.
@@ -218,6 +259,8 @@ Section first_order_terms.
   Fact fo_term_syms_fix_1 s v : fo_term_syms (@in_fot s v) = s::flat_map fo_term_syms (vec_list v).
   Proof. rewrite fo_term_syms_fix_2, vec_list_vec_map, <- flat_map_concat_map; auto. Qed.
 
+  *)
+
 End first_order_terms.
 
 Arguments in_var { var sym sym_ar }.
@@ -228,16 +271,6 @@ Tactic Notation "rew" "fot" := autorewrite with fo_term_db.
 Hint Rewrite fo_term_vars_fix_0 fo_term_vars_fix_1 
              fo_term_syms_fix_0 fo_term_syms_fix_1 : fo_term_db.
 
-Fact flat_map_flat_map X Y Z (f : X -> list Y) (g : Y -> list Z) l : 
-       flat_map g (flat_map f l) = flat_map (fun x => flat_map g (f x)) l.
-Proof.
-  induction l; simpl; auto.
-  rewrite flat_map_app; f_equal; auto.
-Qed.
-
-Fact flat_map_single X Y (f : X -> Y) l : flat_map (fun x => f x::nil) l = map f l.
-Proof. induction l; simpl; f_equal; auto. Qed.
-
 Section fo_term_subst.
 
   Variable (sym : Type) (sym_ar : sym -> nat)
@@ -245,11 +278,22 @@ Section fo_term_subst.
 
   Implicit Type (σ : X -> fo_term Y sym_ar).
 
-  Fixpoint fo_term_subst' σ (t : fo_term X sym_ar) :=
+  Fixpoint fo_term_subst σ (t : fo_term X sym_ar) :=
     match t with 
       | in_var x   => σ x
-      | in_fot s v => in_fot s (vec_map (fo_term_subst' σ) v)
+      | in_fot s v => in_fot s (vec_map (fo_term_subst σ) v)
     end.
+
+  Notation "t ⟬ σ ⟭" := (fo_term_subst σ t).
+
+  Fact fo_term_subst_fix_0 σ x : (in_var x)⟬σ⟭  = σ x.
+  Proof. trivial. Qed.
+
+  Fact fo_term_subst_fix_1 σ s v : (in_fot s v)⟬σ⟭ 
+                                  = in_fot s (vec_map (fo_term_subst σ) v).
+  Proof. trivial. Qed.
+
+  (*
 
   Definition fo_term_subst σ : fo_term X sym_ar -> fo_term Y sym_ar.
   Proof.
@@ -267,25 +311,45 @@ Section fo_term_subst.
                                   = in_fot s (vec_map (fo_term_subst σ) v).
   Proof. apply fo_term_recursion_fix_1. Qed.
 
+  *)
+
   Opaque fo_term_subst.
 
-  Global Hint Rewrite fo_term_subst_fix_0 fo_term_subst_fix_1 : fo_term_db.
+  Hint Rewrite fo_term_subst_fix_0 fo_term_subst_fix_1 : fo_term_db.
 
   Fact fo_term_subst_ext f g t : 
      (forall x, In x (fo_term_vars t) -> f x = g x) -> t⟬f⟭ = t⟬g⟭.
   Proof.
     induction t as [ | s v IHv ]; intros Hfg; rew fot.
     + apply Hfg; rew fot; simpl; auto.
-    + f_equal; apply vec_map_ext.
-      intros; apply IHv; auto.
+    + simpl; f_equal; apply vec_map_ext.
+      intros x Hx. 
+      apply in_vec_list, vec_list_inv in Hx.
+      destruct Hx as (p & ->).
+      apply IHv.
       intros y Hy; apply Hfg; rew fot. 
-      apply in_flat_map; exists x.
-      rewrite <- in_vec_list; tauto.
+      apply in_flat_map; exists (vec_pos v p).
+      split; auto; apply in_vec_list; auto.
   Qed.
 
   Section map.
 
     Variable (f : X -> Y).
+
+    Fixpoint fo_term_map (t : fo_term X sym_ar) := 
+      match t with
+        | in_var x   => in_var (f x)
+        | in_fot s v => in_fot s (vec_map fo_term_map v)
+      end.
+
+    Fact fo_term_map_fix_0 x : fo_term_map (in_var x) = in_var (f x).
+    Proof. trivial. Qed.
+
+    Fact fo_term_map_fix_1 s v : 
+         fo_term_map (in_fot s v) = in_fot s (vec_map fo_term_map v).
+    Proof. trivial. Qed.
+
+    (*
 
     Definition fo_term_map : fo_term X sym_ar -> fo_term Y sym_ar.
     Proof.
@@ -301,6 +365,8 @@ Section fo_term_subst.
          fo_term_map (in_fot s v) = in_fot s (vec_map fo_term_map v).
     Proof. apply fo_term_recursion_fix_1. Qed.
 
+    *)
+
   End map.
 
   Opaque fo_term_map.
@@ -308,7 +374,10 @@ Section fo_term_subst.
   Hint Rewrite fo_term_map_fix_0 fo_term_map_fix_1 : fo_term_db.
 
   Fact fo_term_subst_map f t : t⟬fun x => in_var (f x)⟭ = fo_term_map f t.
-  Proof. induction t; rew fot; f_equal. Qed.
+  Proof. 
+    induction t; rew fot; f_equal.
+    apply vec_pos_ext; intro; rew vec. 
+  Qed.
 
   Fact fo_term_map_ext f g t : (forall x, In x (fo_term_vars t) -> f x = g x)
                              -> fo_term_map f t = fo_term_map g t.
@@ -329,8 +398,9 @@ Section fo_term_subst.
       rewrite flat_map_concat_map, map_map, <- flat_map_concat_map.
       do 2 rewrite flat_map_concat_map; f_equal.
       apply map_ext_in; intros x Hx.
+      apply vec_list_inv in Hx.
+      destruct Hx as (p & ->).
       rewrite IHv; auto.
-      apply in_vec_list; auto.
   Qed.
 
   Fact fo_term_vars_map f t : fo_term_vars (fo_term_map f t) = map f (fo_term_vars t).
@@ -346,17 +416,15 @@ Section fo_term_subst.
     do 2 rewrite flat_map_concat_map; f_equal.
     rewrite vec_list_vec_map, map_map.
     apply map_ext_in.
-    intros x Hx; apply IHv, in_vec_list; auto.
+    intros x Hx; apply vec_list_inv in Hx.
+    destruct Hx as (p & ->); apply IHv.
   Qed.
 
-(*
+  (** The identity is going to be complicated only permutation will do
+      the syms in the substitution are those in the original term + all
+      those occuring in the substitution on the variables in t 
 
-  The identity is going to be complicated only permutation will do
-  the syms in the substitution are those in the original term + all
-  those occuring in the substitution on the variables in t 
-
-  We show the weaker 
-*)
+      We show the weaker  *)
 
   Fact fo_term_syms_subst P f t : 
         (forall n, In n (fo_term_vars t) -> Forall P (fo_term_syms (f n)))  
@@ -370,16 +438,17 @@ Section fo_term_subst.
         intros (s' & H3 & H4).
         rewrite vec_list_vec_map, in_map_iff in H3.
         destruct H3 as (t & <- & H3).
-        apply in_vec_list in H3.
+        apply vec_list_inv in H3.
+        destruct H3 as (p & ->).
         revert x H4; apply Forall_forall, IH; auto.
         - intros; apply H1; rew fot; apply in_flat_map.
-          exists t; split; auto. 
-          apply in_vec_list; auto.
+          exists (vec_pos v p); split; auto. 
+          apply in_vec_list, in_vec_pos.
         - revert H2; do 2 rewrite Forall_forall.
           intros H2 x Hx; apply H2; rew fot.
           right; apply in_flat_map.
-          exists t; split; auto.
-          apply in_vec_list; auto.
+          exists (vec_pos v p); split; auto.
+          apply in_vec_list, in_vec_pos.
   Qed.
 
 End fo_term_subst.
@@ -401,7 +470,7 @@ Section fo_term_subst_comp.
   Proof.
     induction t; rew fot; auto; rew fot.
     rewrite vec_map_map; f_equal.
-    apply vec_map_ext; auto.
+    apply vec_pos_ext; intros p; rew vec.
   Qed.
 
 End fo_term_subst_comp.
@@ -427,6 +496,22 @@ Section semantics.
 
   Implicit Type φ : X -> M.
 
+  Fixpoint fo_term_sem φ (t : 𝕋) :=
+    match t with
+      | in_var x   => φ x
+      | in_fot s v => sem_sym (vec_map (fo_term_sem φ) v)
+    end.
+
+  Notation "⟦ t ⟧" := (fun φ => @fo_term_sem φ t).
+
+  Fact fo_term_sem_fix_0 φ n : ⟦in_var n⟧ φ = φ n.
+  Proof. trivial. Qed.
+
+  Fact fo_term_sem_fix_1 φ s v : ⟦in_fot s v⟧ φ = sem_sym (vec_map (fun t => ⟦t⟧ φ) v).
+  Proof. trivial. Qed.
+
+  (*
+
   Definition fo_term_sem φ : 𝕋 -> M.
   Proof.
     induction 1 as [ x | s _ w ] using fo_term_recursion.
@@ -442,6 +527,8 @@ Section semantics.
   Fact fo_term_sem_fix_1 φ s v : ⟦in_fot s v⟧ φ = sem_sym (vec_map (fun t => ⟦t⟧ φ) v).
   Proof. apply fo_term_recursion_fix_1. Qed.
 
+  *)
+
   Opaque fo_term_sem.
 
   Hint Rewrite fo_term_sem_fix_0 fo_term_sem_fix_1 : fo_term_db.
@@ -449,20 +536,22 @@ Section semantics.
   Fact fo_term_sem_ext t φ ψ : 
         (forall n, In n (fo_term_vars t) -> φ n = ψ n) -> ⟦t⟧ φ = ⟦t⟧ ψ.
   Proof.
-    revert φ ψ; induction t as [ n | s v IHv ]; intros phi psy H; rew fot.
+    induction t as [ n | s v IHv ] in φ, ψ |- *; intros H; rew fot.
     + apply H; simpl; auto.
     + f_equal; apply vec_map_ext.
-      intros x Hx; apply IHv; auto.
+      intros x Hx.
+      apply in_vec_list, vec_list_inv in Hx.
+      destruct Hx as (p & ->).
+      apply IHv; auto.
       intros n Hn; apply H; rew fot.
-      apply in_flat_map; exists x; split; auto.
+      apply in_flat_map; exists (vec_pos v p); split; auto.
       apply in_vec_list; auto.
   Qed.
 
   Fact fo_term_sem_subst φ σ t : ⟦t⟬σ⟭⟧ φ = ⟦t⟧ (fun n => ⟦σ n⟧ φ).
   Proof.
     induction t; rew fot; f_equal; auto.
-    rewrite vec_map_map.
-    apply vec_map_ext; intros; auto.
+    apply vec_pos_ext; intros; rew vec.
   Qed.
 
 End semantics.
@@ -480,11 +569,24 @@ Section rel_semantics.
 
   Implicit Type φ : X -> M -> Prop.
 
-  Fixpoint fo_term_rsem' φ (t : 𝕋) : M -> Prop :=
+  Fixpoint fo_term_rsem φ (t : 𝕋) : M -> Prop :=
     match t with
       | in_var x   => φ x
-      | in_fot s v => fun m => exists w, @sem_sym s w m /\ forall p, fo_term_rsem' φ (vec_pos v p) (vec_pos w p)
+      | in_fot s v => fun m => exists w, @sem_sym s w m /\ forall p, fo_term_rsem φ (vec_pos v p) (vec_pos w p)
     end.
+
+  Notation "⟦ t ⟧" := (fun φ => @fo_term_rsem φ t).
+
+  Fact fo_term_rsem_fix_0 φ n : ⟦in_var n⟧ φ = φ n.
+  Proof. trivial. Qed.
+
+  Fact fo_term_rsem_fix_1 φ s v r : 
+           ⟦in_fot s v⟧ φ r 
+       <-> exists w, @sem_sym s w r 
+                  /\ forall p, ⟦vec_pos v p⟧ φ (vec_pos w p).
+  Proof. simpl; tauto. Qed.
+
+  (*
 
   Definition fo_term_rsem φ : 𝕋 -> M -> Prop.
   Proof.
@@ -512,6 +614,8 @@ Section rel_semantics.
     apply fol_equiv_ext; auto.
   Qed.
 
+  *)
+
   Opaque fo_term_rsem.
 
   Hint Rewrite fo_term_rsem_fix_0 fo_term_rsem_fix_1 : fo_term_db.
@@ -519,7 +623,7 @@ Section rel_semantics.
   Fact fo_term_rsem_ext t φ ψ : 
         (forall n r, In n (fo_term_vars t) -> φ n r <-> ψ n r) -> forall r, ⟦t⟧ φ r <-> ⟦t⟧ ψ r.
   Proof.
-    revert φ ψ; induction t as [ n | s v IHv ] using fo_term_pos_rect; intros phi psy H; rew fot.
+    induction t as [ n | s v IHv ] in φ, ψ |- *; intros H; rew fot.
     + intro; apply H; simpl; auto.
     + intros r; rew fot.
       apply exists_equiv; intros w.
@@ -529,7 +633,7 @@ Section rel_semantics.
       intros; apply H; rew fot.
       apply in_flat_map.
       exists (vec_pos v p); split; auto.
-      apply in_vec_list, in_vec_pos.
+      apply in_vec_list; auto.
   Qed.
 
 End rel_semantics.
@@ -546,7 +650,7 @@ Section equiv.
   Theorem fo_term_sem_rsem_equiv (t : fo_term X sym_ar) φ r : 
            r = fo_term_sem sM φ t <-> fo_term_rsem (fun s v r => r = @sM s v) (fun n r => r = φ n) t r.
   Proof.
-    revert φ r; induction t as [ n | s v IHv ] using fo_term_pos_rect; intros phi r; rew fot; try tauto.
+    revert φ r; induction t as [ n | s v IHv ]; intros phi r; rew fot; try tauto.
     split.
     + intros ->.
       exists (vec_map (fo_term_sem sM phi) v); split; auto.
@@ -580,7 +684,7 @@ Section rel_simulation.
                                                                                          /\ forall p, vec_pos v p ⋈ vec_pos w p)   
           -> forall x y, x ⋈ y -> fo_term_rsem sM φ t x <-> fo_term_rsem sN ψ t y.
   Proof.
-    induction t as [ n | s v IHv ] using fo_term_pos_rect; intros H1 H2 H2' x y Hxy; rew fot; try tauto.
+    induction t as [ n | s v IHv ]; intros H1 H2 H2' x y Hxy; rew fot; try tauto.
     + apply H1; simpl; auto.
     + split.
       * intros (v' & H3 & H4).
